post-cip/formal-crypto/lean/src/Leioscrypto/Vote.lean
@@ -12,6 +12,8 @@ inductive Vote where
 | PersistentVote : ElectionId → PoolIndex → BlockHash → BLS.Signature → Vote
 | NonpersistentVote : ElectionId → PoolKeyHash → BLS.Signature → BlockHash → BLS.Signature → Vote
 
+-- TODO: Create a valid vote.
+
 namespace Vote
 
   def electionId : Vote → ElectionId
